Experiment with new module-based interface to LN backend

Tealeaves/Backends/LN.v
@@ -1,1 +1,339 @@
-From Tealeaves.Backends.LN Require Export Atom AtomSet AssocList LN.
+From Tealeaves.Backends.LN Require Export
+  Atom AtomSet AssocList LN.
+
+From Tealeaves.Misc Require Import
+  NaturalNumbers.
+From Tealeaves.Theory Require Import
+  DecoratedTraversableMonad.
+
+Module Type SyntaxSIGHetero.
+  Parameter (iterm oterm : Type).
+  Parameter (T U : Type -> Type).
+  Parameter ret_inst: Return T.
+  Parameter binddt_T_inst: Binddt nat T T.
+  Parameter binddt_U_inst: Binddt nat T U.
+  Parameter module_inst:
+    DecoratedTraversableRightModule nat T U
+      (Return_inst := ret_inst)
+      (Bindd_T_inst := binddt_T_inst)
+      (Bindd_U_inst := binddt_U_inst)
+      (unit := Monoid_unit_zero)
+      (op := Monoid_op_plus).
+  Parameter to_T:  iterm -> T LN.
+  Parameter to_T_inv: T LN -> iterm.
+  Parameter to_U: oterm -> U LN.
+  Parameter to_U_inv: U LN -> oterm.
+  Parameter to_T_iso : forall (t : iterm), to_T_inv (to_T t) = t.
+  Parameter to_U_iso : forall (t : oterm), to_U_inv (to_U t) = t.
+  Parameter to_T_iso_inv : forall (t : T LN), to_T (to_T_inv t) = t.
+  Parameter to_U_iso_inv : forall (t : U LN), to_U (to_U_inv t) = t.
+  Parameter from_atom: atom -> iterm.
+  Parameter from_ix: nat -> iterm.
+  Parameter from_atom_Ret:
+    from_atom = to_T_inv ○ @ret T ret_inst LN ○ Fr.
+  Parameter from_ix_Ret:
+    from_ix = to_T_inv ○ @ret T ret_inst LN ○ Bd.
+End SyntaxSIGHetero.
+
+Module Type TheorySIG.
+  Parameters iterm oterm : Type.
+  Parameters
+    (open : iterm -> oterm -> oterm)
+    (close : atom -> oterm -> oterm)
+    (subst : atom -> iterm -> oterm -> oterm)
+    (locally_closed_b : oterm -> bool).
+End TheorySIG.
+
+Module MakeTheory_Hetero
+  (Syntax: SyntaxSIGHetero) <: TheorySIG.
+  Import Syntax.
+
+  Definition iterm := Syntax.iterm.
+  Definition oterm := Syntax.oterm.
+
+  #[local] Existing Instance Syntax.ret_inst.
+  #[local] Existing Instance Syntax.binddt_T_inst.
+  #[local] Existing Instance Syntax.binddt_U_inst.
+  #[local] Existing Instance Syntax.module_inst.
+  #[local] Existing Instance Map_Binddt.
+  #[local] Existing Instance Mapd_Binddt.
+  #[local] Existing Instance Traverse_Binddt.
+  #[local] Existing Instance Mapdt_Binddt.
+  #[local] Existing Instance Bind_Binddt.
+  #[local] Existing Instance Bindt_Binddt.
+  #[local] Existing Instance Bindd_Binddt.
+
+  Import AtomSet.Notations.
+
+  Coercion to_T : Syntax.iterm >-> T.
+  Coercion to_U : Syntax.oterm >-> U.
+
+  Definition open : iterm -> oterm -> oterm :=
+    fun t u => to_U_inv (open (T := T) (U := U) t u).
+
+  Definition close : atom -> oterm -> oterm :=
+    fun x u => to_U_inv (close (T := U) x u).
+
+  Definition subst : atom -> iterm -> oterm -> oterm :=
+    fun x t u => to_U_inv (subst (T := T) (U := U) x t u).
+
+  Definition free : oterm -> list atom :=
+    fun u => free (T := U) u.
+
+  Definition freeset : oterm -> AtomSet.t :=
+    fun u => freeset (T := U) u.
+
+  Definition locally_closed : oterm -> Prop :=
+    fun u => locally_closed (U := U) u.
+
+  Definition locally_closed_b : oterm -> bool :=
+    fun u => locally_closed_b (U := U) u.
+
+  Definition scoped : oterm -> AtomSet.t -> Prop :=
+    fun t γ => freeset t ⊆ γ.
+
+  Definition subst_i : atom -> iterm -> iterm -> iterm :=
+    fun x t u => to_T_inv (LN.subst (T := T) (U := T) x t u).
+
+  Definition freeset_i : iterm -> AtomSet.t :=
+    fun t => LN.freeset (T := T) t.
+
+  Definition locally_closed_i : iterm -> Prop :=
+    fun u => LN.locally_closed (U := T) u.
+
+  Module Notations.
+    Notation "t '{ x ~> u }" := (subst x u t) (at level 35).
+    Notation "t '( u )" := (open u t) (at level 35).
+    Notation "'[ x ] t" := (close x t) (at level 35).
+  End Notations.
+
+  Import Notations.
+
+  Coercion from_atom : atom >-> Syntax.iterm.
+  Coercion from_ix : nat >-> Syntax.iterm.
+
+  Implicit Types (x y: atom) (t: iterm) (u: oterm).
+
+  Theorem open_lc: forall t u,
+      locally_closed u -> u '(t) = u.
+  Proof.
+    intros.
+    unfold locally_closed.
+    unfold open.
+    rewrite open_lc.
+    - apply to_U_iso.
+    - assumption.
+  Qed.
+
+  Theorem freeset_subst_upper: forall x t u,
+      freeset (u '{x ~> t}) ⊆ freeset u \\ {{x}} ∪ freeset_i t.
+  Proof.
+    intros.
+    unfold freeset, freeset_i, subst.
+    rewrite to_U_iso_inv.
+    rewrite freeset_subst_upper.
+    reflexivity.
+  Qed.
+
+  Theorem freeset_subst_lower: forall t u x,
+      freeset u \\ {{ x }} ⊆ freeset (u '{x ~> t}).
+  Proof.
+    intros.
+    unfold freeset, freeset_i, subst.
+    rewrite to_U_iso_inv.
+    apply freeset_subst_lower.
+  Qed.
+
+  Theorem close_open : forall x u,
+      ~ x ∈@ freeset u ->
+      '[x] (u '(from_atom x)) = u.
+  Proof.
+    intros.
+    unfold close, open.
+    rewrite from_atom_Ret.
+    rewrite to_U_iso_inv.
+    rewrite to_T_iso_inv.
+    rewrite close_open.
+    - rewrite to_U_iso.
+      reflexivity.
+    - rewrite free_iff_freeset.
+      assumption.
+  Qed.
+
+  Theorem open_close : forall x u,
+      ('[x] u) '(x) = u.
+  Proof.
+    intros.
+    unfold close, open.
+    rewrite from_atom_Ret.
+    rewrite to_U_iso_inv.
+    rewrite to_T_iso_inv.
+    rewrite open_close.
+    rewrite to_U_iso.
+    reflexivity.
+  Qed.
+
+  Theorem subst_open_var : forall u t x y,
+      x <> y ->
+      locally_closed_i t ->
+      u '(from_atom y) '{x ~> t} =
+        u '{x ~> t} '(from_atom y).
+  Proof.
+    intros.
+    unfold close, open, subst.
+    rewrite to_U_iso_inv.
+    rewrite to_U_iso_inv.
+    rewrite from_atom_Ret.
+    rewrite to_T_iso_inv.
+    rewrite subst_open_var.
+    - reflexivity.
+    - assumption.
+    - assumption.
+  Qed.
+
+  Theorem open_spec_eq : forall u t x,
+      ~ x ∈@ freeset u ->
+      u '(t) = u '(from_atom x) '{x ~> t}.
+  Proof.
+    intros.
+    unfold close, open, subst.
+    rewrite to_U_iso_inv.
+    erewrite open_spec_eq.
+    - rewrite from_atom_Ret.
+      rewrite to_T_iso_inv.
+      reflexivity.
+    - assumption.
+  Qed.
+
+  Theorem subst_open :  forall t1 t2 u x,
+      locally_closed_i t2 ->
+      u '(t1) '{x ~> t2} =
+        open (subst_i x t2 t1) (u '{x ~> t2}).
+  Proof.
+    intros.
+    unfold close, open, subst, subst_i.
+    rewrite to_U_iso_inv.
+    rewrite subst_open.
+    - rewrite to_U_iso_inv.
+      rewrite to_T_iso_inv.
+      reflexivity.
+    - assumption.
+  Qed.
+
+  Theorem freeset_open_upper : forall u t,
+      freeset (u '(t)) ⊆ freeset u ∪ freeset_i t.
+  Proof.
+    intros.
+    unfold freeset, open.
+    rewrite to_U_iso_inv.
+    rewrite freeset_open_upper.
+    reflexivity.
+  Qed.
+
+  Theorem freeset_open_lower : forall t u,
+      freeset u ⊆ freeset (u '(t)).
+  Proof.
+    intros.
+    unfold freeset, open.
+    rewrite to_U_iso_inv.
+    rewrite freeset_open_lower.
+    reflexivity.
+  Qed.
+
+  Theorem freeset_close : forall u x,
+      freeset ('[x] u) [=] freeset u \\ {{ x }}.
+  Proof.
+    intros.
+    unfold freeset, close.
+    rewrite to_U_iso_inv.
+    rewrite freeset_close.
+    reflexivity.
+  Qed.
+
+  Theorem nin_freeset_close : forall u x,
+      ~ x ∈@ freeset ('[x] u).
+  Proof.
+    intros.
+    unfold freeset, close.
+    rewrite to_U_iso_inv.
+    apply nin_freeset_close.
+  Qed.
+
+  Theorem freeset_close1 : forall u x y,
+      y <> x ->
+      y ∈@ freeset ('[x] u) <-> y ∈@ freeset u.
+  Proof.
+    intros.
+    unfold close, freeset.
+    rewrite to_U_iso_inv.
+    rewrite <- free_iff_freeset.
+    rewrite in_free_close_iff.
+    rewrite <- free_iff_freeset.
+    intuition.
+  Qed.
+
+End MakeTheory_Hetero.
+
+Module Type SyntaxSIG.
+  Parameter (term : Type).
+  Parameter (T : Type -> Type).
+  Parameter
+    (ret_inst : Return T)
+    (binddt_inst : Binddt nat T T)
+    (monad_inst : DecoratedTraversableMonad nat T
+              (unit := Monoid_unit_zero)
+              (op := Monoid_op_plus)).
+  Parameter to_T:  term -> T LN.
+  Parameter to_T_inv: T LN -> term.
+  Parameter to_T_iso : forall (t : term), to_T_inv (to_T t) = t.
+  Parameter to_T_iso_inv : forall (t : T LN), to_T (to_T_inv t) = t.
+  Parameter from_atom: atom -> term.
+  Parameter from_ix: nat -> term.
+  Parameter from_atom_Ret:
+    from_atom = to_T_inv ○ @ret T ret_inst LN ○ Fr.
+  Parameter from_ix_Ret:
+    from_ix = to_T_inv ○ @ret T ret_inst LN ○ Bd.
+End SyntaxSIG.
+
+Module Adapter (M1: SyntaxSIG) <: SyntaxSIGHetero.
+
+  Definition iterm := M1.term.
+  Definition oterm := M1.term.
+  Definition T := M1.T.
+  Definition U := M1.T.
+  Definition ret_inst := M1.ret_inst.
+  Definition binddt_T_inst := M1.binddt_inst.
+  Definition binddt_U_inst := M1.binddt_inst.
+  Definition module_inst :=
+    @DecoratedTraversableRightModule_DecoratedTraversableMonad
+      nat T _ _ M1.ret_inst M1.binddt_inst M1.monad_inst.
+  Definition to_T := M1.to_T.
+  Definition to_T_inv := M1.to_T_inv.
+  Definition to_T_iso := M1.to_T_iso.
+  Definition to_T_iso_inv := M1.to_T_iso_inv.
+  Definition to_U := M1.to_T.
+  Definition to_U_inv := M1.to_T_inv.
+  Definition to_U_iso := M1.to_T_iso.
+  Definition to_U_iso_inv := M1.to_T_iso_inv.
+  Definition from_atom := M1.from_atom.
+  Definition from_ix := M1.from_ix.
+  Definition from_atom_Ret := M1.from_atom_Ret.
+  Definition from_ix_Ret := M1.from_ix_Ret.
+
+End Adapter.
+
+Module MakeTheory (Syntax: SyntaxSIG) <:
+    (TheorySIG with Definition iterm := Syntax.term
+     with Definition oterm := Syntax.term).
+
+  Module Syntax_Hetero <: SyntaxSIGHetero
+  := Adapter Syntax.
+
+  Module Theory <:
+    (TheorySIG with Definition iterm := Syntax.term
+     with Definition oterm := Syntax.term)
+    := MakeTheory_Hetero Syntax_Hetero.
+
+  Include Theory.
+
+End MakeTheory.
