Tealeaves/Examples/STLC/CompatTest.v
@@ -1,0 +1,131 @@
+From Tealeaves Require Export
+  Backends.LN
+  Misc.NaturalNumbers
+  Functors.List
+  Theory.DecoratedTraversableMonad
+  Examples.STLC.Syntax.
+
+Export Kleisli.DecoratedTraversableMonad.Notations. (* ∈d *)
+Import Monoid.Notations. (* Ƶ and ● *)
+Import Misc.Subset.Notations. (* ∪ *)
+Export Applicative.Notations. (* <⋆> *)
+Export List.ListNotations. (* [] :: *)
+Export LN.Notations. (* operations *)
+Export LN.AtomSet.Notations.
+Export LN.AssocList.Notations. (* one, ~ *)
+Export Product.Notations. (* × *)
+Export ContainerFunctor.Notations. (* ∈ *)
+Export DecoratedContainerFunctor.Notations. (* ∈d *)
+
+#[local] Generalizable Variables G.
+
+#[local] Set Implicit Arguments.
+
+(** * Language definition *)
+(******************************************************************************)
+Inductive term :=
+| atm : atom -> term
+| ix  : nat -> term
+| lam : typ -> term -> term
+| app : term -> term -> term.
+
+(** ** Notations and automation *)
+(******************************************************************************)
+Module Notations.
+  Notation "'fun'" := (lam) (at level 45).
+  Notation "[ t1 ]@[ t2 ]" := (app t1 t2) (at level 80).
+  Notation "A ⟹ B" := (arr A B) (at level 40).
+End Notations.
+
+Import Notations.
+
+(** ** Instantiate Tealeaves *)
+(******************************************************************************)
+Fixpoint to_T (t: term) : Syntax.term LN :=
+  match t with
+  | atm a => Syntax.tvar (Fr a)
+  | ix n => Syntax.tvar (Bd n)
+  | lam τ t => Syntax.lam τ (to_T t)
+  | app t1 t2 => Syntax.app (to_T t1) (to_T t2)
+  end.
+
+Fixpoint to_T_inv (t: Syntax.term LN) : term :=
+  match t with
+  | tvar (Fr a) => atm a
+  | tvar (Bd n) => ix n
+  | Syntax.lam τ t => lam τ (to_T_inv t)
+  | Syntax.app t1 t2 => app (to_T_inv t1) (to_T_inv t2)
+  end.
+
+Lemma to_T_iso: forall (t : term), to_T_inv (to_T t) = t.
+Proof.
+  intros.
+  induction t.
+  - reflexivity.
+  - reflexivity.
+  - cbn. now rewrite IHt.
+  - cbn. now rewrite IHt1, IHt2.
+Qed.
+
+Lemma to_T_iso_inv: forall (t : Syntax.term LN), to_T (to_T_inv t) = t.
+Proof.
+  intros.
+  induction t.
+  - cbn. destruct v; reflexivity.
+  - cbn. now rewrite IHt.
+  - cbn. now rewrite IHt1, IHt2.
+Qed.
+
+Module STLC_SIG <: SyntaxSIG with Definition term := term.
+
+  Definition term : Type := term.
+  Definition T := Syntax.term.
+  Definition ret_inst := Syntax.Return_STLC.
+  Definition binddt_inst := Syntax.Binddt_STLC.
+  Definition monad_inst := Syntax.DTM_STLC.
+
+  Definition to_T := to_T.
+  Definition to_T_inv := to_T_inv.
+  Definition to_T_iso := to_T_iso.
+  Definition to_T_iso_inv := to_T_iso_inv.
+
+  Definition from_atom := atm.
+  Definition from_ix := ix.
+
+  Definition from_atom_Ret:
+    from_atom = to_T_inv ○ @ret T ret_inst LN ○ Fr :=
+    ltac:(reflexivity).
+  Definition from_ix_Ret:
+    from_ix = to_T_inv ○ @ret T ret_inst LN ○ Bd :=
+    ltac:(reflexivity).
+
+End STLC_SIG.
+
+Module Theory <: TheorySIG
+  := MakeTheory STLC_SIG.
+Import Theory.
+Import Theory.Notations.
+
+(** ** Deeper Instantiate Tealeaves *)
+(******************************************************************************)
+
+(** ** Use Tealeaves *)
+(******************************************************************************)
+Reserved Notation "Γ ⊢ t : S" (at level 90, t at level 99).
+
+Inductive Judgment : ctx -> term -> typ -> Prop :=
+| j_var :
+    forall (Γ : ctx) (x : atom) (A : typ),
+      uniq Γ ->
+      (x, A) ∈ Γ ->
+      Γ ⊢ (atm x) : A
+| j_abs :
+    forall (L : AtomSet.t) Γ (τ1 τ2: typ) (t: term),
+      (forall x : atom, ~ AtomSet.In x L -> Γ ++ x ~ τ1 ⊢ t '(atm x) : τ2) ->
+      Γ ⊢ fun τ1 t : τ1 ⟹ τ2
+| j_app :
+    forall Γ (t1 t2 : term) (A B : typ),
+      Γ ⊢ t1 : A ⟹ B ->
+      Γ ⊢ t2 : A ->
+      Γ ⊢ [t1]@[t2] : B
+where "Γ ⊢ t : A" := (Judgment Γ t A).
