Tealeaves/Misc/Prop.v
@@ -20,3 +20,32 @@ Solve All Obligations with intros; propext; firstorder.
   @Monoid_Morphism Prop Prop or False and True not.
 
 Solve Obligations with intros; propext; firstorder.
+
+(** * Boolean monoids *)
+#[export] Instance Monoid_op_bool_or: Monoid_op bool := orb.
+
+#[export] Instance Monoid_unit_bool_false: Monoid_unit bool := false.
+
+#[program, export] Instance Monoid_disjunction_bool: @Monoid bool orb false.
+
+Next Obligation.
+  now destruct x, y, z.
+Qed.
+
+Next Obligation.
+  now destruct x.
+Qed.
+
+#[export] Instance Monoid_op_bool_and: Monoid_op bool := andb.
+
+#[export] Instance Monoid_unit_bool_true: Monoid_unit bool := true.
+
+#[program, export] Instance Monoid_conjunction_bool: @Monoid bool andb true.
+
+Next Obligation.
+  now destruct x, y, z.
+Qed.
+
+Next Obligation.
+  now destruct x.
+Qed.
